extra/Decode.v
@@ -1,0 +1,154 @@
+
+(* ********************************************************************** *)
+(* * Decoders *)
+
+(* ---------------------------------------------------------------------- *)
+(* ** [Decode] predicate and instances *)
+
+Definition Decode (v:val) A {EA:Enc A} (V:A) : Prop :=
+  v = ``V.
+
+Lemma Decode_enc : forall A (EA:Enc A) (V:A),
+  Decode (``V) V.
+Proof using. intros. hnfs~. Qed.
+
+Hint Extern 1 (Decode (``_) _) => eapply Decode_enc : Decode.
+
+Lemma Decode_unit :
+  Decode val_unit tt.
+Proof using. intros. hnfs~. Qed.
+
+Lemma Decode_int : forall (n:int),
+  Decode (val_int n) n.
+Proof using. intros. hnfs~. Qed.
+
+Lemma Decode_bool : forall (b:bool),
+  Decode (val_bool b) b.
+Proof using. intros. hnfs~. Qed.
+
+Lemma Decode_loc : forall (l:loc),
+  Decode (val_loc l) l.
+Proof using. intros. hnfs~. Qed.
+
+Hint Resolve Decode_unit Decode_int Decode_bool Decode_loc : Decode.
+
+Lemma Decode_nil : forall A (EA:Enc A),
+  Decode (val_constr "nil" nil) (@nil A).
+Proof using. intros. hnfs~. Qed.
+
+Lemma Decode_cons : forall A (EA:Enc A) (X:A) (L:list A) (x l : val),
+  Decode x X ->
+  Decode l L ->
+  Decode (val_constr "cons" (x::l::nil)) (X::L).
+Proof using. introv Dx DL. unfolds. rew_enc. fequals. Qed.
+
+Lemma Decode_None : forall A (EA:Enc A),
+  Decode (val_constr "none" nil) (@None A).
+Proof using. intros. hnfs~. Qed.
+
+Lemma Decode_Some : forall A (EA:Enc A) (V:A) (v:val),
+  Decode v V ->
+  Decode (val_constr "some" (v::nil)) (Some V).
+Proof using. intros. unfolds. rew_enc. fequals. Qed.
+
+(* TODO: generalize to tuples, and strings and char base types *)
+
+(* ---------------------------------------------------------------------- *)
+(* ** Predicate [Decodes] *)
+
+Definition Decodes (vs:vals) (Vs:dyns) : Prop :=
+  vs = encs Vs.
+
+Lemma Decodes_nil :
+  Decodes nil nil.
+Proof using. intros. hnfs~. Qed.
+
+Lemma Decodes_cons : forall (v:val) (vs:vals) A (EA:Enc A) (V:A) (Vs:dyns),
+  Decode v V ->
+  Decodes vs Vs ->
+  Decodes (v::vs) ((Dyn V)::Vs).
+Proof using.
+  introv Dv Dvs. unfolds Decodes. simpl. rewrite enc_dyn_make. fequals.
+Qed.
+
+
+
+Lemma Triple_ref_Decode : forall A (EA:Enc A) (V:A) (v:val),
+  Decode v V ->
+  Triple (val_ref v)
+    \[]
+    (fun l => l ~~> V).
+Proof using. introv Hv. unfolds Decode. subst v. applys Triple_ref. Qed.
+
+
+
+
+Lemma Triple_set_Decode : forall A1 `{EA1:Enc A1} (V1 V2:A1) (l:loc) (v2:val),
+  Decode v2 V2 ->
+  Triple (val_set l v2)
+    (l ~~> V1)
+    (fun (u:unit) => l ~~> V2).
+Proof using.
+  introv Hv2. unfolds Decode. subst v2. applys Triple_set.
+Qed.
+Lemma Triple_eq_Decode : forall A `(EA:Enc A) (v1 v2:val) (V1 V2:A),
+  Decode v1 V1 ->
+  Decode v2 V2 ->
+  Enc_comparable V1 V2 ->
+  Triple (val_eq v1 v2)
+    \[]
+    (fun (b:bool) => \[b = isTrue (V1 = V2)]).
+Proof using.
+  introv D1 D2 I. unfolds Decode. subst v1 v2. applys* Triple_eq.
+Qed.
+
+
+Lemma Triple_neq_Decode : forall A `(EA:Enc A) (v1 v2:val) (V1 V2:A),
+  Decode v1 V1 ->
+  Decode v2 V2 ->
+  Enc_comparable V1 V2 ->
+  Triple (val_neq v1 v2)
+    \[]
+    (fun (b:bool) => \[b = isTrue (V1 <> V2)]).
+Proof using.
+  introv D1 D2 I. unfolds Decode. subst v1 v2. applys* Triple_neq.
+Qed.
+
+
+
+Hint Extern 1 (Register_Spec (val_set_field _)) => Provide @Triple_set_field_Decode.
+
+(* not used
+Lemma xapp_record_new_noarg : forall (Vs:dyns) (Q:loc->hprop) (H:hprop) (ks:fields) (vs:vals),
+  noduplicates_fields_exec ks = true ->
+  LibListExec.is_nil ks = false ->
+  Decodes vs Vs ->
+  List.length ks = List.length Vs ->
+  (fun p => p ~> Record (List.combine ks Vs)) \*+ H ===> (protect Q) ->
+  H ==> ^(Wpgen_app_untyped (trm_apps (trm_val (val_record_init ks)) (trms_vals vs))) Q.
+Proof using. introv HN HE HD EQ HI. unfolds Decodes. applys* xapp_record_new. Qed.
+*)
+
+(* DEPRECATED
+Ltac xnew_core_noarg tt :=
+  applys xapp_record_new_noarg;
+  [ try reflexivity
+  | try reflexivity
+  | xdecodes
+  | try reflexivity
+  | xsimpl; simpl List.combine; unfold protect; xnew_post tt ].
+
+Ltac xapp_record_new tt :=
+  xnew_core_noarg tt.
+
+Tactic Notation "xnew" :=
+  xnew_core_noarg tt.
+*)
+
+
+Lemma Triple_set_field_Decode : forall (v2:val) A (EA:Enc A) (V1:A) (l:loc) f (V2:A),
+  Decode v2 V2 ->
+  Triple ((val_set_field f) l v2)
+    (l`.f ~~> V1)
+    (fun (r:unit) => l`.f ~~> V2).
+Proof using. introv M. unfolds Decode. subst v2. applys Triple_set_field_strong. Qed.
